compiler/core/Driver/CompLang.v
@@ -65,7 +65,7 @@ Section CompLang.
     | L_nnrs_core : language
     | L_nnrs : language
     | L_nnrs_imp : language
-    | L_imp_qcert : language
+    | L_imp_data : language
     | L_imp_ejson : language
     | L_nnrcmr : language
     | L_dnnrc : language
@@ -111,7 +111,7 @@ Section CompLang.
       | "nnrs_core"%string => L_nnrs_core
       | "nnrs"%string => L_nnrs
       | "nnrs_imp"%string => L_nnrs_imp
-      | "imp_qcert"%string => L_imp_qcert
+      | "imp_data"%string => L_imp_data
       | "imp_ejson"%string => L_imp_ejson
       | "nnrcmr"%string => L_nnrcmr
       | "dnnrc"%string => L_dnnrc
@@ -142,7 +142,7 @@ Section CompLang.
       | L_nnrs_core => "nnrs_core"%string
       | L_nnrs => "nnrs"%string
       | L_nnrs_imp => "nnrs_imp"%string
-      | L_imp_qcert => "imp_qcert"%string
+      | L_imp_data => "imp_data"%string
       | L_imp_ejson => "imp_ejson"%string
       | L_nnrcmr => "nnrcmr"%string
       | L_dnnrc => "dnnrc"%string
@@ -203,7 +203,7 @@ Section CompLang.
         :: (L_nnrs_core,BackEnd,"cNNRS", "Core Named Nested Relational Calculus imperative")
         :: (L_nnrs,CoreEnd,"NNRS", "Named Nested Relational Calculus imperative")
         :: (L_nnrs_imp,BackEnd,"NNRSimp", "Named Nested Relational Calculus imperative")
-        :: (L_imp_qcert,BackEnd,"ImpQcert", "Imperative langauge with Q*cert data model")
+        :: (L_imp_data,BackEnd,"ImpData", "Imperative langauge with Q*cert data model")
         :: (L_imp_ejson,BackEnd,"ImpJson", "Imperative langauge with json data model")
         :: (L_nnrcmr,DistrEnd,"NNRCMR", "Named Nested Relational Calculus with Map/Reduce")
         :: (L_dnnrc,DistrEnd,"DNNRC", "Distributed Named Nested Relational Calculus")
@@ -299,9 +299,9 @@ Section CompLang.
     Definition nnrs_imp_expr := nnrs_imp_expr.
     Definition nnrs_imp_stmt := nnrs_imp_stmt.
     Definition nnrs_imp := nnrs_imp.
-    Definition imp_qcert_expr := imp_qcert_expr.
-    Definition imp_qcert_stmt := imp_qcert_stmt.
-    Definition imp_qcert := imp_qcert.
+    Definition imp_data_expr := imp_data_expr.
+    Definition imp_data_stmt := imp_data_stmt.
+    Definition imp_data := imp_data.
     Definition imp_ejson := imp_ejson.
     Definition nnrcmr := nnrcmr.
     Definition dnnrc := dnnrc.
@@ -328,7 +328,7 @@ Section CompLang.
     | Q_nnrs_core : nnrs_core -> query
     | Q_nnrs : nnrs -> query
     | Q_nnrs_imp : nnrs_imp -> query
-    | Q_imp_qcert : imp_qcert -> query
+    | Q_imp_data : imp_data -> query
     | Q_imp_ejson : imp_ejson -> query
     | Q_nnrcmr : nnrcmr -> query
     | Q_dnnrc : dnnrc -> query
@@ -357,7 +357,7 @@ Section CompLang.
       | Case_aux c "Q_nnrs_core"%string
       | Case_aux c "Q_nnrs"%string
       | Case_aux c "Q_nnrs_imp"%string
-      | Case_aux c "Q_imp_qcert"%string
+      | Case_aux c "Q_imp_data"%string
       | Case_aux c "Q_imp_ejson"%string
       | Case_aux c "Q_nnrcmr"%string
       | Case_aux c "Q_dnnrc"%string
@@ -386,7 +386,7 @@ Section CompLang.
       | Q_nnrs_core _ => L_nnrs_core
       | Q_nnrs _ => L_nnrs
       | Q_nnrs_imp _ => L_nnrs_imp
-      | Q_imp_qcert _ => L_imp_qcert
+      | Q_imp_data _ => L_imp_data
       | Q_imp_ejson _ => L_imp_ejson
       | Q_nnrcmr _ => L_nnrcmr
       | Q_dnnrc _ => L_dnnrc
@@ -421,7 +421,7 @@ Section CompLang.
       | L_nnrs_core => nnrs_core
       | L_nnrs => nnrs
       | L_nnrs_imp => nnrs_imp
-      | L_imp_qcert => imp_qcert
+      | L_imp_data => imp_data
       | L_imp_ejson => imp_ejson
       | L_nnrcmr => nnrcmr
       | L_dnnrc => dnnrc
@@ -454,7 +454,7 @@ Tactic Notation "language_cases" tactic(first) ident(c) :=
   | Case_aux c "L_nnrs_core"%string
   | Case_aux c "L_nnrs"%string
   | Case_aux c "L_nnrs_imp"%string
-  | Case_aux c "L_imp_qcert"%string
+  | Case_aux c "L_imp_data"%string
   | Case_aux c "L_imp_ejson"%string
   | Case_aux c "L_nnrcmr"%string
   | Case_aux c "L_dnnrc"%string
