compiler/core/Imp/Lang/ImpDataEval.v
@@ -33,46 +33,46 @@ Require Import Utils.
 Require Import DataRuntime.
 Require Import Imp.
 Require Import ImpEval.
-Require Import ImpQcert.
+Require Import ImpData.
 
-Section ImpQcertEval.
+Section ImpDataEval.
   Context {fruntime:foreign_runtime}.
 
   Context (h:brand_relation_t).
 
-  (* Local Open Scope imp_qcert. *)
+  (* Local Open Scope imp_data. *)
   Local Open Scope string.
   Import ListNotations.
 
   Section EvalInstantiation.
-    (* Instantiate Imp for Qcert data *)
-    Definition imp_qcert_data_normalize (d:imp_qcert_data) : imp_qcert_data :=
+    (* Instantiate Imp for Data data *)
+    Definition imp_data_data_normalize (d:imp_data_data) : imp_data_data :=
       normalize_data h d.
 
-    Definition imp_qcert_data_to_bool (d:imp_qcert_data) : option bool :=
+    Definition imp_data_data_to_bool (d:imp_data_data) : option bool :=
       match d with
       | dbool b => Some b
       | _ => None
       end.
 
-    Definition imp_qcert_data_to_Z (d:imp_qcert_data) : option Z :=
+    Definition imp_data_data_to_Z (d:imp_data_data) : option Z :=
       match d with
       | dnat n => Some n
       | _ => None
       end.
 
-    Definition imp_qcert_Z_to_data (n:Z) : imp_qcert_data :=
+    Definition imp_data_Z_to_data (n:Z) : imp_data_data :=
       dnat n.
 
-    Definition imp_qcert_data_to_list (d:imp_qcert_data) : option (list imp_qcert_data) :=
+    Definition imp_data_data_to_list (d:imp_data_data) : option (list imp_data_data) :=
       match d with
       | dcoll c => Some (c)
       | _ => None
       end.
 
-    Definition imp_qcert_runtime_eval (rt:imp_qcert_runtime_op) (dl:list imp_qcert_data) : option imp_qcert_data :=
+    Definition imp_data_runtime_eval (rt:imp_data_runtime_op) (dl:list imp_data_data) : option imp_data_data :=
       match rt with
-      | QcertRuntimeGroupby g kl =>
+      | DataRuntimeGroupby g kl =>
         match dl with
         | (dcoll dl) :: nil =>
           match group_by_nested_eval_table g kl dl with
@@ -81,33 +81,33 @@ Section ImpQcertEval.
           end
         | _ => None
         end
-      | QcertRuntimeEither =>
+      | DataRuntimeEither =>
         match dl with
         | (dleft d) :: nil => Some (dbool true)
         | (dright d) :: nil => Some (dbool false)
         | _ => None
         end
-      | QcertRuntimeToLeft =>
+      | DataRuntimeToLeft =>
         match dl with
         | (dleft d) :: nil => Some d
         | _ => None
         end
-      | QcertRuntimeToRight =>
+      | DataRuntimeToRight =>
         match dl with
         | (dright d) :: nil => Some d
         | _ => None
         end
       end.
 
-    Definition imp_qcert_op_eval (op:imp_qcert_op) (dl:list imp_qcert_data) : option imp_qcert_data :=
+    Definition imp_data_op_eval (op:imp_data_op) (dl:list imp_data_data) : option imp_data_data :=
       match op with
-      | QcertOpUnary uop =>
+      | DataOpUnary uop =>
         match dl with
         | [d] =>
           unary_op_eval h uop d
         | _ => None
         end
-      | QcertOpBinary bop =>
+      | DataOpBinary bop =>
         match dl with
         | [d1;d2] =>
           binary_op_eval h bop d1 d2
@@ -120,88 +120,88 @@ Section ImpQcertEval.
   (** ** Evaluation Semantics *)
   Section Evaluation.
 
-    (** Evaluation takes a ImpQcert expression and an environment. It
+    (** Evaluation takes a ImpData expression and an environment. It
           returns an optional value. When [None] is returned, it
           denotes an error. An error is always propagated. *)
 
-    Definition imp_qcert_expr_eval
-             (σ:pd_bindings) (e:imp_qcert_expr)
+    Definition imp_data_expr_eval
+             (σ:pd_bindings) (e:imp_data_expr)
     : option data
       := @imp_expr_eval
-           imp_qcert_data
-           imp_qcert_op
-           imp_qcert_runtime_op
-           imp_qcert_data_normalize
-           imp_qcert_runtime_eval
-           imp_qcert_op_eval
+           imp_data_data
+           imp_data_op
+           imp_data_runtime_op
+           imp_data_data_normalize
+           imp_data_runtime_eval
+           imp_data_op_eval
            σ e.
 
-    Definition imp_qcert_decls_eval
-               (σ:pd_bindings) (el:list (string * option imp_qcert_expr))
+    Definition imp_data_decls_eval
+               (σ:pd_bindings) (el:list (string * option imp_data_expr))
       : option pd_bindings
       := @imp_decls_eval
-           imp_qcert_data
-           imp_qcert_op
-           imp_qcert_runtime_op
-           imp_qcert_data_normalize
-           imp_qcert_runtime_eval
-           imp_qcert_op_eval
+           imp_data_data
+           imp_data_op
+           imp_data_runtime_op
+           imp_data_data_normalize
+           imp_data_runtime_eval
+           imp_data_op_eval
            σ el.
 
-    Definition imp_qcert_decls_erase
-               (σ:option pd_bindings) (el:list (string * option imp_qcert_expr))
+    Definition imp_data_decls_erase
+               (σ:option pd_bindings) (el:list (string * option imp_data_expr))
       : option pd_bindings
       := imp_decls_erase σ el.
 
-    Definition imp_qcert_stmt_eval
-             (s:imp_qcert_stmt) (σ:pd_bindings) : option (pd_bindings)
+    Definition imp_data_stmt_eval
+             (s:imp_data_stmt) (σ:pd_bindings) : option (pd_bindings)
       := @imp_stmt_eval
-           imp_qcert_data
-           imp_qcert_op
-           imp_qcert_runtime_op
-           imp_qcert_data_normalize
-           imp_qcert_data_to_bool
-           imp_qcert_data_to_Z
-           imp_qcert_data_to_list
-           imp_qcert_Z_to_data
-           imp_qcert_runtime_eval
-           imp_qcert_op_eval
+           imp_data_data
+           imp_data_op
+           imp_data_runtime_op
+           imp_data_data_normalize
+           imp_data_data_to_bool
+           imp_data_data_to_Z
+           imp_data_data_to_list
+           imp_data_Z_to_data
+           imp_data_runtime_eval
+           imp_data_op_eval
            s σ.
 
-    Definition imp_qcert_function_eval
-             (f:imp_qcert_function) args : option imp_qcert_data
+    Definition imp_data_function_eval
+             (f:imp_data_function) args : option imp_data_data
       := @imp_function_eval
-           imp_qcert_data
-           imp_qcert_op
-           imp_qcert_runtime_op
-           imp_qcert_data_normalize
-           imp_qcert_data_to_bool
-           imp_qcert_data_to_Z
-           imp_qcert_data_to_list
-           imp_qcert_Z_to_data
-           imp_qcert_runtime_eval
-           imp_qcert_op_eval
+           imp_data_data
+           imp_data_op
+           imp_data_runtime_op
+           imp_data_data_normalize
+           imp_data_data_to_bool
+           imp_data_data_to_Z
+           imp_data_data_to_list
+           imp_data_Z_to_data
+           imp_data_runtime_eval
+           imp_data_op_eval
            f args.
 
-    Definition imp_qcert_eval (q:imp_qcert) (d: data) : option (option data)
+    Definition imp_data_eval (q:imp_data) (d: data) : option (option data)
       := @imp_eval
-           imp_qcert_data
-           imp_qcert_op
-           imp_qcert_runtime_op
-           imp_qcert_data_normalize
-           imp_qcert_data_to_bool
-           imp_qcert_data_to_Z
-           imp_qcert_data_to_list
-           imp_qcert_Z_to_data
-           imp_qcert_runtime_eval
-           imp_qcert_op_eval
+           imp_data_data
+           imp_data_op
+           imp_data_runtime_op
+           imp_data_data_normalize
+           imp_data_data_to_bool
+           imp_data_data_to_Z
+           imp_data_data_to_list
+           imp_data_Z_to_data
+           imp_data_runtime_eval
+           imp_data_op_eval
            q d.
 
-    Definition imp_qcert_eval_top σc (q:imp_qcert) :=
-      olift id (imp_qcert_eval q (drec (rec_sort σc))).
+    Definition imp_data_eval_top σc (q:imp_data) :=
+      olift id (imp_data_eval q (drec (rec_sort σc))).
 
   End Evaluation.
 
-End ImpQcertEval.
+End ImpDataEval.
 
 (* Arguments imp_stmt_eval_domain_stack {fruntime h s σ₁ σ₂}. *)
