compiler/core/Imp/Lang/ImpData.v
@@ -1,0 +1,54 @@
+(*
+ * Licensed under the Apache License, Version 2.0 (the "License");
+ * you may not use this file except in compliance with the License.
+ * You may obtain a copy of the License at
+ *
+ * http://www.apache.org/licenses/LICENSE-2.0
+ *
+ * Unless required by applicable law or agreed to in writing, software
+ * distributed under the License is distributed on an "AS IS" BASIS,
+ * WITHOUT WARRANTIES OR CONDITIONS OF ANY KIND, either express or implied.
+ * See the License for the specific language governing permissions and
+ * limitations under the License.
+ *)
+
+(** Imp with the Q*cert data model *)
+
+Require Import String.
+Require Import Utils.
+Require Import DataRuntime.
+Require Import Imp.
+
+Section ImpData.
+  Context {fruntime:foreign_runtime}.
+  Section Syntax.
+
+    Definition imp_data_data := data.
+
+    Inductive imp_data_op :=
+    | DataOpUnary : unary_op -> imp_data_op
+    | DataOpBinary : binary_op -> imp_data_op
+    .
+
+    Inductive imp_data_runtime_op :=
+    | DataRuntimeGroupby : string -> list string -> imp_data_runtime_op
+    | DataRuntimeEither : imp_data_runtime_op
+    | DataRuntimeToLeft : imp_data_runtime_op
+    | DataRuntimeToRight : imp_data_runtime_op
+    .
+
+    Definition imp_data_expr := @imp_expr imp_data_data imp_data_op imp_data_runtime_op.
+    Definition imp_data_stmt := @imp_stmt imp_data_data imp_data_op imp_data_runtime_op.
+    Definition imp_data_function := @imp_function imp_data_data imp_data_op imp_data_runtime_op.
+    Definition imp_data := @imp imp_data_data imp_data_op imp_data_runtime_op.
+  End Syntax.
+
+End ImpData.
+
+Tactic Notation "imp_data_runtime_op_cases" tactic(first) ident(c) :=
+  first;
+  [ Case_aux c "DataRuntimeGroupby"%string
+  | Case_aux c "DataRuntimeEither"%string
+  | Case_aux c "DataRuntimeLeft"%string
+  | Case_aux c "DataRuntimeRight"%string
+  ].
